(WIP) Defining refinement

Behaviors.v
@@ -2,14 +2,24 @@ Require Import Common.
 Require Import State.
 Require Import Value.
 Require Import BinNat.
+Require Import Memory.
+Require Import sflib.
+Require Import Omega.
 
-(* Defines what a program behavior is. *)
+(* This file defines what a program behavior is. *)
+
 
 Module Ir.
 
 Inductive event :=
 | e_none: event
-| e_some (v:Ir.val): event.
+| e_some (n:N): event.
+
+Definition not_none (e:event): bool :=
+  match e with
+  | e_none => false
+  | _ => true
+  end.
 
 (* Trace is a list of events. *)
 Definition trace := list event.
@@ -26,14 +36,48 @@ Inductive program_behavior :=
 .
 
 
-Definition refines_trace (tr_tgt tr_src:trace) :=
-  
+Definition refines_value (v_tgt v_src:Ir.val): bool :=
+  match (v_tgt, v_src) with
+  | (_, Ir.poison) => true
+  | (Ir.num ntgt, Ir.num nsrc) => N.eqb ntgt nsrc
+  | (Ir.ptr ptgt, Ir.ptr psrc) => Ir.ptr_eqb ptgt psrc
+  | (_, _) => false
+  end.
+
+Definition refines_event (e_tgt e_src:event): bool :=
+  match (e_tgt, e_src) with
+  | (e_some vtgt, e_some vsrc) => N.eqb vtgt vsrc
+  | (e_none, e_none) => true
+  | _ => false
+  end.
+
+Definition refines_trace (tr_tgt tr_src:trace):bool :=
+  let tr_tgt' := List.filter not_none tr_tgt in
+  let tr_src' := List.filter not_none tr_src in
+  if Nat.eqb (List.length tr_tgt') (List.length tr_src') then
+    List.forallb (fun ee => refines_event ee.(fst) ee.(snd))
+                 (List.combine tr_tgt' tr_src')
+  else false.
+
+(* If tgts_prefix is true, check whether tr_tgt has a prefix
+   that refines tr_src.
+   If tgts_prefix is false, check whether tr_src has a prefix
+   so tr_tgt refines the prefix. *)
+Definition refines_trace_prefix (tr_tgt tr_src:trace) (tgts_prefix:bool)
+: bool :=
+  let tr_tgt' := List.filter not_none tr_tgt in
+  let tr_src' := List.filter not_none tr_src in
+  let (tr_tgt', tr_src') :=
+      if tgts_prefix then (List.firstn (List.length tr_src') tr_tgt', tr_src')
+      else (tr_tgt', List.firstn (List.length tr_tgt') tr_src') in
+  refines_trace tr_tgt' tr_src'.
+
 
 (* Checks whether the behavior of a target program refines the behavior of a source program. *)
 Definition refines (pb_tgt pb_src:program_behavior):bool :=
   match (pb_tgt, pb_src) with
   | (b_terminates tr_tgt ret_tgt, b_terminates tr_src ret_src) =>
-    refines_trace tr_tgt tr_src && refines_val ret_tgt ret_src
+    refines_trace tr_tgt tr_src && refines_value ret_tgt ret_src
 
   | (b_terminates tr_tgt ret_tgt, b_diverges tr_src) =>
     (* infinite loop without any event is UB.
@@ -71,9 +115,68 @@ Definition refines (pb_tgt pb_src:program_behavior):bool :=
 
   | (b_oom tr_tgt, b_oom tr_src) =>
     (* target trace should be prefix of source trace. *)
-    refines_trace_prefix tr_tgt tr_src
+    refines_trace_prefix tr_tgt tr_src true
 
   | (_, _) => false
   end.
+
+
+
+Theorem refines_value_refl:
+  forall (v:Ir.val), refines_value v v = true.
+Proof.
+  intros.
+  destruct v; unfold refines_value.
+  - rewrite N.eqb_eq. auto.
+  - rewrite Ir.ptr_eqb_refl. reflexivity.
+  - reflexivity.
+Qed.
+
+Theorem refines_event_refl:
+  forall (e:event), refines_event e e = true.
+Proof.
+  intros.
+  destruct e. unfold refines_event. reflexivity.
+  unfold refines_event. rewrite N.eqb_eq. reflexivity.
+Qed.
+
+Theorem refines_trace_refl:
+  forall (t:trace), refines_trace t t = true.
+Proof.
+  intros.
+  induction t.
+  - reflexivity.
+  - unfold refines_trace in *.
+    assert (forall {X:Type} (l:list X), (List.length l =? List.length l) = true).
+    { intros.
+      rewrite Nat.eqb_eq. reflexivity. }
+    rewrite H. rewrite H in IHt.
+    simpl.
+    destruct (not_none a) eqn:HNN.
+    simpl. rewrite IHt. rewrite refines_event_refl. reflexivity.
+    assumption.
+Qed.
+
+Theorem refines_trace_prefix_refl:
+  forall (t:trace) b, refines_trace_prefix t t b = true.
+Proof.
+  intros.
+  destruct b; unfold refines_trace_prefix in *;
+    rewrite List.firstn_all in *;
+    rewrite refines_trace_refl;
+    reflexivity.
+Qed.
+
+Theorem refines_refl:
+  forall (pb:program_behavior), refines pb pb = true.
+Proof.
+  intros.
+  destruct pb; unfold refines.
+  - rewrite refines_trace_refl.
+    rewrite refines_value_refl. reflexivity.
+  - rewrite refines_trace_refl. reflexivity.
+  - rewrite refines_trace_refl. reflexivity.
+  - rewrite refines_trace_prefix_refl. reflexivity.
+Qed.
 
 End Ir.
